1  x=5 y=2 z=3 m=1 n=4   x * y – z*2
2  x=5 y=2 z=3 m=1 n=4   17– y * 7 + n
3  x=5 y=2 z=3 m=1 n=4   n * z + x *y
4  x=5 y=2 z=3 m=1 n=4   z+ y* (13 - 9)
5  x=5 y=2 z=3 m=1 n=4   28- (x - m) -z
6  x=5 y=2 z=3 m=1 n=4   22 +x * (n- m)
7  x=5 y=2 z=3 m=1 n=4   37 + 9 - z :m *x
8  x=5 y=2 z=3 m=1 n=4   18 : (11 - x) +y
9  x=5 y=2 z=3 m=1 n=4   x*n-(16+z)
10 x=5 y=2 z=3 m=1 n=4   n:y+z*y
11 A=8  B=4 C=1 D=3      (A/B-C)*D+B
12 A=8  B=4 C=1 D=3      (A+B-C)*D
13 A=8  B=4 C=1 D=3      (A/B+C)*D-A
14 A=8  B=4 C=1 D=3      (A-B/C)*D
15 A=8  B=4 C=1 D=3      (A/B-C)*D
16 A=8  B=4 C=1 D=3      (A/B+D-C)*D
17 A=8  B=4 C=1 D=3      (A/B-C)*D+A
18 A=8  B=4 C=1 D=3      (A/B-C)*D+C
19 A=8  B=4 C=1 D=3      (A/B-C)*D-C
20 A=8  B=4 C=1 D=3      (A/B-C)*D+D
